theories/EqProps.v
@@ -1,0 +1,35 @@
+Set Primitive Projections.
+From Equations Require Import Equations.
+
+From Paco Require Import paco.
+From OGS Require Import Utils Ctx EventD CatD ITreeD EqD RecD AngelicD.
+
+Record observing {I} {E : event I I} {X Y : psh I}
+           (R : forall i, itree' E X i -> itree' E Y i -> Prop)
+           i (t1 : itree E X i) (t2 : itree E Y i) : Prop :=
+  observing_intros
+  { observing_observe : R _ (observe t1) (observe t2) }.
+Global Hint Constructors observing: core.
+
+
+Lemma unfold_iter {I} {E : event I I} {X Y : I -> Type}
+           (f : X ⇒ᵢ itree E (X +ᵢ Y)) {i} (x : X i) 
+           : observing eqᵢ _
+              (iter f i x)
+              (bind (f i x) (fun i y => match y with
+                                        | inl x => Tau (iter f i x)
+                                        | inr y => Ret y
+                                        end)).
+constructor; reflexivity.
+Qed.
+
+Lemma unfold_iterₐ {I} {E : event I I} {X Y i}
+           (f : X -> itreeₐ E i i (X + Y)) (x : X)
+  : observing eqᵢ _
+      (iterₐ f x)
+      (f x !>= fun r => match r with
+                     | inl x => tauₐ (iterₐ f x)
+                     | inr y => retₐ y
+                     end).
+constructor; reflexivity.
+Qed.
